theories/SmallStep.v
@@ -2,9 +2,9 @@ From LinearCore Require
   Context
   Match
   NewNames
-  Rename
   Shape
   Term
+  Unshadow
   UsedIn
   .
 From LinearCore Require Import
@@ -61,17 +61,11 @@ Inductive Step (context : Context.context) : Term.term -> Context.context -> Ter
       body_if_match other_cases other_used (scan_other_used
         (* Note that this removes already bound terms, since `UsedIn` won't shadow: *)
         : Map.Reflect (UsedIn.Term (Term.App (Term.Cas pattern body_if_match other_cases) scrutinee)) other_used)
-      to_self_other (other_idem : Map.ToSelf other_used to_self_other)
-      reserved (union_into_reserved : Map.Union (Map.domain context) other_used reserved)
-      new_names (generate_new_names : NewNames.generate reserved (BoundIn.pattern pattern) = new_names)
-      name_map (merge_names : Map.BulkOverwrite new_names to_self_other name_map) (O2O : Map.OneToOne name_map)
-      renamed_pattern (rename_pattern : Rename.Pattern O2O pattern renamed_pattern)
-      renamed_body_if_match (rename_body_if_match : Rename.Term O2O body_if_match renamed_body_if_match)
-      renamed_other_cases (rename_other_cases : Rename.Term O2O other_cases renamed_other_cases)
+      context_or_used (union_into_context_or_used : Map.Union (Map.domain context) other_used context_or_used)
+      renamed (rename : Unshadow.unshadow context_or_used
+        (Term.App (Term.Cas pattern body_if_match other_cases) scrutinee) = Some renamed)
       unchanged_context (context_unchanged : Map.Eq context unchanged_context)
-      : Step context
-        (Term.App (Term.Cas pattern body_if_match other_cases) scrutinee) unchanged_context
-        (Term.App (Term.Cas renamed_pattern renamed_body_if_match renamed_other_cases) scrutinee)
+      : Step context (Term.App (Term.Cas pattern body_if_match other_cases) scrutinee) unchanged_context renamed
     .
 Arguments Step context term updated_context updated_term.
 
@@ -142,17 +136,16 @@ Proof.
       * destruct N as [x [U B]]. edestruct safe_names. { exact U. } exact B.
     + split. { eapply Map.eq_trans. { apply Map.eq_sym. exact context_unchanged. }
         eapply Map.eq_trans. { exact Ec. } exact context_unchanged0. }
-      eassert (eq_name_map : Map.Eq name_map name_map0). 2: { f_equal. f_equal;
-        [eapply Rename.pattern_det | eapply Rename.term_det | eapply Rename.term_det];
-        try reflexivity; try eassumption; exact eq_name_map. }
-      eassert (eq_other : Map.Eq other_used other_used0). {
-        intros k []. split; intro F; (eassert (I : Map.In _ _); [eexists; exact F |]);
+      assert (Eou : Map.Eq other_used other_used0). {
+        split; intro F; (eassert (I : Map.In _ _); [eexists; exact F |]);
         [apply scan_other_used in I | apply scan_other_used0 in I];
         [apply scan_other_used0 in I | apply scan_other_used in I];
-        destruct I as [[] F']; exact F'. }
-      eapply Map.bulk_overwrite_det; try eassumption. 2: { eapply Map.to_self_det; eassumption. }
-      erewrite NewNames.generate_det; try apply Map.eq_refl. eapply Map.union_det; try eassumption.
-      intros k []. repeat rewrite Map.find_domain. apply Map.in_eq. exact Ec.
+        destruct v; destruct I as [[] F']; exact F'. }
+      assert (Ecu : Map.Eq context_or_used context_or_used0). {
+        eapply Map.union_det; try eassumption. split; intro F; apply Map.find_domain;
+        apply Map.find_domain in F; (eapply Map.in_eq; [| exact F]); [apply Map.eq_sym |]; exact Ec. }
+      destruct (@Unshadow.det _ _ Ecu (Term.App (Term.Cas pattern body_if_match other_cases) scrutinee) _ eq_refl).
+      rewrite rename0 in rename. invert rename. reflexivity.
 Qed.
 
 
@@ -165,19 +158,19 @@ Lemma eq
   {t2'} (Et' : t1' = t2')
   : Step c2 t2 c2' t2'.
 Proof.
-  subst. rename t2 into t. rename t2' into t'. generalize dependent c2'. generalize dependent c2. {
-  induction S1; cbn in *; intros.
+  subst. rename t2 into t. rename t2' into t'. generalize dependent c2'. generalize dependent c2.
+  induction S1; intros.
   - constructor. { apply Ec. exact lookup. } destruct no_contraction as [I R]. split.
     + eapply Map.in_eq. { apply Map.eq_sym. exact Ec. } eexists. exact lookup.
-    + intros x y. rewrite <- Ec'. rewrite <- Ec. apply R.
+    + cbn in *. intros x y. rewrite <- Ec'. rewrite <- Ec. apply R.
   - econstructor.
     + apply Ec. exact lookup.
     + destruct remove_self_from_context as [I R]. split.
       * eapply Map.in_eq. { apply Map.eq_sym. exact Ec. } exact I.
-      * intros x y. rewrite R. rewrite Ec. reflexivity.
+      * cbn in *. intros x y. rewrite R. rewrite Ec. reflexivity.
     + exact S1.
     + exact not_overwriting_self.
-    + intros x y. rewrite <- Ec'. apply update.
+    + cbn in *. intros x y. rewrite <- Ec'. apply update.
   - constructor.
     + eapply Match.compatible_eq; try reflexivity; eassumption.
     + intros. eapply safe_names; eassumption.
@@ -198,33 +191,13 @@ Proof.
       eapply Map.eq_trans. { exact context_unchanged. } exact Ec'.
   - econstructor.
     + destruct not_yet_safe_to_match as [N | [x [U B]]]; [left | right].
-      * intro C. apply N. eapply Match.compatible_eq. { exact C. } 2: { reflexivity. }
+      * intro C. apply N. eapply Match.compatible_eq. 3: { reflexivity. } { exact C. }
         apply Map.eq_sym. exact Ec.
       * exists x. split. { exact U. } exact B.
     + exact scan_other_used.
-    + eassumption.
-    + intros x y. rewrite union_into_reserved. fold (Map.domain context). repeat rewrite Map.find_domain.
-      erewrite Map.in_eq. { reflexivity. } exact Ec.
-    + eassumption.
-    + eassumption.
-    + eassumption.
-    + eassumption.
-    + eassumption.
-    + eapply Map.eq_trans. { apply Map.eq_sym. exact Ec. }
-      eapply Map.eq_trans. { exact context_unchanged. } exact Ec'. }
+    + intros k v. unfold Map.Union in union_into_context_or_used. rewrite union_into_context_or_used.
+      split; (intros [F | F]; [left | right; exact F]); apply Map.find_domain;
+      apply Map.find_domain in F; (eapply Map.in_eq; [| exact F]); [apply Map.eq_sym |]; exact Ec.
+    + assumption.
+    + eapply Map.eq_trans. { apply Map.eq_sym. exact Ec. } eapply Map.eq_trans. { exact context_unchanged. } exact Ec'.
 Qed.
-
-
-
-Theorem name_invariant {context term updated_context updated_term}
-  (original_stepped : Step context term updated_context updated_term)
-  {name_mappings} (O2O : Map.OneToOne name_mappings)
-  {renamed_term} (rename_term : Rename.Term O2O term renamed_term)
-  {renamed_context} (rename_context : Rename.Context O2O context renamed_context)
-  : exists updated_renamed_context updated_renamed_term,
-    Step renamed_context renamed_term updated_renamed_context updated_renamed_term /\
-    exists updated_name_mappings (O2OU : Map.OneToOne updated_name_mappings),
-      Rename.Term O2OU updated_term updated_renamed_term /\
-      Rename.Context O2OU updated_context updated_renamed_context.
-Proof.
-Abort.
